src/KInduction.v
@@ -2,32 +2,15 @@ Require Export Bmc.Core.
 Require Import Omega.
 
 
-Definition k_violate_loop_free (I : init) (T : trans)
+Definition k_ind_step (I : init) (T : trans)
   (P : prop) (k: nat) : Prop :=
   forall ss : sseq,
   ~ (loop_free T ss 0 k /\ safety_k_offset P ss 0 k /\ ~ P ss.[k]).
 
-
 Definition k_induction_post (I : init) (T : trans) (P : prop) (k: nat) : Prop :=
-  k_violate_loop_free I T P k /\ safety_k I T P k.
+  k_ind_step I T P k /\ safety_k I T P k.
 
 (**)
-
-Lemma safety_prop_k_init : 
-  forall (i k : nat) (I : init) (T : trans) (P : prop),
-  (i < k) -> safety_k I T P k -> prop_k_init I T P i.
-Proof.
-  intros * H H0.
-  induction k.
-  - easy.
-  - destruct (Nat.lt_ge_cases i k) as [H1|H1].
-    + assert (safety_k I T P k /\ prop_k_init I T P k) as A
-      by (destruct k; firstorder; now rewrite <- plus_n_O in H0).
-      now apply (IHk H1). 
-    + apply gt_S_le in H.
-      assert (i = k) as A by omega.
-      destruct k; rewrite A; firstorder.
-Qed.
 
 Lemma skipn_safety_k_offset : 
   forall (P : prop) (i j : nat) (ss : sseq),
@@ -50,15 +33,15 @@ Proof.
       destruct i; firstorder.
 Qed.
 
-Lemma shift_violate_loop_free : 
+Lemma shift_k_ind_step : 
   forall (T : trans) (P : prop) (i k : nat),
-  S k <= i ->
+  k < i ->
   ( forall ss : sseq,
-     ~ ( loop_free T ss 0 (S k) /\ 
-         safety_k_offset P ss 0 (S k) /\ ~ P ss.[S k] )) ->
+     ~ ( loop_free T ss 0 k /\ 
+         safety_k_offset P ss 0 k /\ ~ P ss.[k] )) ->
   forall ss : sseq,
-  ~ ( loop_free T ss (i-k-1) (S k) /\ 
-    safety_k_offset P ss (i-k-1) (S k) /\ ~ (P (ss.[i])) ).
+  ~ ( loop_free T ss (i-k) k /\ 
+    safety_k_offset P ss (i-k) k /\ ~ (P (ss.[i])) ).
 Proof.
   intros * H H0 *.
   apply neg_false.
@@ -69,25 +52,21 @@ Proof.
     destruct H1 as [H1 H1'].
     destruct H2 as [H2 H2'].
     apply skipn_no_loop in H1'.
-    apply skipn_prop with (k := S k) in H2'.
+    apply skipn_prop with (k := k) in H2'.
     apply skipn_path in H1.
     apply skipn_safety_k_offset in H2.
-    replace (i - S k) with (i - k - 1) in H2'.
-
-    assert (( path T (skipn (i - k - 1) ss) 0 (S k) /\
-      no_loop (skipn (i - k - 1) ss) 0 (S k) ) /\
-      safety_k_offset P (skipn (i - k - 1) ss) 0 (S k) /\ 
-      ~ P (skipn (i - k - 1) ss).[S k] ) as A
+    assert (( path T (skipn (i-k) ss) 0 k /\
+      no_loop (skipn (i-k) ss) 0 k ) /\
+      safety_k_offset P (skipn (i-k) ss) 0 k /\ 
+      ~ P (skipn (i-k) ss).[k] ) as A
       by firstorder.
-
     apply H0 in A.
     contradiction.
-    omega.
     omega.
   - tauto.
 Qed.
 
-Lemma divide_hd_all_prop : forall (P : prop) (ss : sseq) (i j : nat),
+Lemma cons_safety_k_offset : forall (P : prop) (ss : sseq) (i j : nat),
   P ss.[i] /\ safety_k_offset P ss (S i) j <->
   safety_k_offset P ss i (S j).
 Proof.
@@ -106,25 +85,17 @@ Qed.
 Lemma lt_wf_ind_incl_prop : 
   forall (I : init) (T : trans) (P : prop) (ss : sseq) (i k : nat),
   k < i -> I ss.[0] /\ loop_free T ss 0 i ->
-  ( forall m : nat, m < i -> I ss.[0] /\ 
-    loop_free T ss 0 m -> P ss.[m] ) -> 
-      safety_k_offset P ss (i-k-1) (S k).
+  ( forall m : nat,
+    m < i -> I ss.[0] /\ loop_free T ss 0 m ->
+    P ss.[m] ) -> 
+      safety_k_offset P ss (i-k) k.
 Proof.
   intros * H H0 H1.
   induction k as [|k IHk].
   - unfold safety_k_offset.
-    split; auto.
-    rewrite -> Nat.sub_0_r.
-    rewrite -> Nat.add_0_r.
-    apply H1.
-    omega.
-    destruct i as [|i].
-    + firstorder.
-    + replace (S i - 1) with i.
-      destruct i; firstorder.
-      omega.
-  - apply divide_hd_all_prop.
-    replace (S (i - S k - 1)) with (i - k - 1).
+    easy.
+  - apply cons_safety_k_offset.
+    replace (i - S k) with (i - k - 1).
     split.
     + apply H1.
       omega.
@@ -132,28 +103,17 @@ Proof.
       * tauto.
       * destruct H0 as [H0 H0'].
         unfold loop_free in *.
-        assert (i = (i - S k - 1) + (k + 2)) as A by omega.
+        assert (i = (i - k - 1) + (k + 1)) as A by omega.
         rewrite A in H0'.
         destruct H0' as [H2 H3].
         apply split_path in H2.
         apply split_no_loop in H3.
         tauto.
-    + apply IHk.
+    + replace (S (i-k-1)) with (i-k).
+      apply IHk.
+      omega.
       omega.
     + omega.
-Qed.
-
-Lemma univ_init_prop : forall (P : prop) (i : nat) (ss : sseq),
-  (forall ss',  ~~ P ss'.[ 0]) -> ~~ P ss.[i].
-Proof.
-  intros * H.
-  assert (forall p : Prop, p -> ~~ p) as A by tauto.
-  apply A.
-  assert (i = i + 0) as A0 by omega.
-  rewrite A0.
-  rewrite <- skipn_nth.
-  apply NNPP.
-  auto.
 Qed.
 
 (**)
@@ -165,48 +125,40 @@ Theorem soundness_k_induction' :
 Proof.
   unfold prop_k_init_lf.
   intros * H *.
-  assert (forall A B C : Prop, (A /\ B -> C) <->  ~ (A /\ B /\ ~ C)) as A by (split; tauto).
-  apply A.
+  apply and_imply_not_and3.
   intros.
 
   induction i as [* H1] using lt_wf_ind.
   unfold k_induction_post in H.
-  destruct (Nat.lt_ge_cases i k) as [H2|H2].
-  - apply safety_prop_k_init with (I:=I) (T:=T) (P:=P) in H2.
+
+  destruct (Nat.le_gt_cases i k) as [H2|H2].
+  - apply bounded_safety with (I:=I) (T:=T) (P:=P) in H2.
     unfold prop_k_init in H2.
-    assert (~ (I ss.[0] /\ path T ss 0 i /\ ~ P ss.[i])) as A0 by auto.
+    assert (~ (I ss.[0] /\ path T ss 0 i /\ ~ P ss.[i])) as A0 by apply H2.
     clear H2.
-    apply <- A in A0.
-    tauto.
+    apply <- and_imply_not_and3 in A0.
+    apply A0.
     firstorder.
     tauto.
   - destruct H as [H H3].
-    unfold k_violate_loop_free in H.
-    destruct k.
-    + unfold loop_free in H.
-      simpl in *.
-      assert (forall ss, ~~ P ss.[0]) as A0 by firstorder.
-      apply univ_init_prop with (i:=i) (ss:=ss) in A0.
-      tauto.
-    + destruct H0 as [H0 H0'].
-      assert (i = (i - k - 1) + (k + 1)) as A0 by omega.
-
-      assert (loop_free T ss 0 i) as A1 by auto.
-      rewrite A0 in A1; clear A0.
-      apply split_loop_free in A1.
-      destruct A1 as [A1 A1'].
-      assert (k < i) as A2 by omega.
-      apply shift_violate_loop_free with
-        (T:=T) (P:=P) (ss:=ss) in H2.
-      apply lt_wf_ind_incl_prop with
-        (I:=I) (T:=T) (P:=P) (ss:=ss) in A2.
-      apply A in H2.
-      auto.
-      rewrite Nat.add_1_r in A1'.
-      auto.
-      auto.
-      auto.
-      auto.
+    unfold k_ind_step in H.
+    destruct H0 as [H0 H0'].
+    assert (i = (i - k) + k) as A0 by omega.
+    assert (loop_free T ss 0 i) as A1 by auto.
+    rewrite A0 in A1; clear A0.
+    apply split_loop_free in A1.
+    destruct A1 as [A1 A1'].
+    assert (k < i) as A2 by omega.
+    apply shift_k_ind_step with
+      (T:=T) (P:=P) (ss:=ss) in H2.
+    apply lt_wf_ind_incl_prop with
+      (I:=I) (T:=T) (P:=P) (ss:=ss) in A2.
+    apply and_imply_not_and3 in H2.
+    apply H2.
+    auto.
+    auto.
+    auto.
+    auto.
 Qed.
 
 Theorem soundness_k_induction :
