src/Forward_example.v
@@ -13,7 +13,7 @@ Goal forward_post ex1_I ex1_T ex1_P 4.
 Proof.
   unfold ex1_I, ex1_T, ex1_P.
   unfold forward_post.
-  unfold lasso.
+  unfold lasso_fwd.
   unfold safety_k.
   unfold prop_k_init.
   unfold loop_free.
@@ -46,7 +46,7 @@ Qed.
 Goal forward_post ex2_I ex2_T ex2_P 3.
 Proof.
   unfold ex2_I, ex2_T, ex2_P.
-  unfold forward_post, lasso, safety_k, prop_k_init, loop_free, path, no_loop, no_loop', sseq, nth, state.
+  unfold forward_post, lasso_fwd, safety_k, prop_k_init, loop_free, path, no_loop, no_loop', sseq, nth, state.
   repeat rewrite -> Nat.add_0_l;
   repeat rewrite -> Nat.add_0_r.
   split.
@@ -57,7 +57,7 @@ Qed.
 Goal forward_post ex3_I ex3_T ex3_P 6.
 Proof.
   unfold ex3_I, ex3_T, ex3_P.
-  unfold forward_post, lasso, violate_loop_free, safety_k, prop_k_init, loop_free, path, no_loop, no_loop', sseq, nth, state.
+  unfold forward_post, lasso_fwd, safety_k, prop_k_init, loop_free, path, no_loop, no_loop', sseq, nth, state.
   repeat rewrite -> Nat.add_0_l;
   repeat rewrite -> Nat.add_0_r.
   split.
